theories/spec.v
@@ -1,81 +1,231 @@
-From stdpp Require Import ssreflect unstable.bitvector.
-From theories Require Import rom.
+(*|
+===================
+Atari Specification
+===================
 
+In this file, I specify the behavior of the Atari 2600.
+I then use this specification to define the *claim* that Dragster cannot be beaten in less than 5.57 seconds.
+
+Since the goal of this project is to prove that something *isn't* possible, I *overapproximate* the behavior of the Atari.
+So my spec might say something is possible even if it isn't, but it will never say something is impossible if it actually is.
+
+As this file defines the thing we are proving, it is the one thing that is not formally verified.
+This is a weakness in this proof — if I've misstated the behavior of the Atari, the proof doesn't prove what I think it does.
+But I would expect such an error to cause a big enough impact to completely mess up the proof, which would mean I would've noticed it.
+
+This weakness could be ameliorated by proving a relationship between this specification and the `http://www.visual6502.org/` netlist.
+But I don't know how to properly specify the set of possible behaviors of a transistor circuit.
+
+--------------
+Bits and Bytes
+--------------
+
+A `bitvector library <https://plv.mpi-sws.org/coqdoc/stdpp/stdpp.unstable.bitvector.html>` is provided by ``std++``, but there are a few things that bother me.
+|*)
+
+From stdpp Require Import ssreflect unstable.bitvector.
 Local Open Scope bv.
 
-Definition bit {n} i (w : bv n) : bool := Z.testbit (bv_unsigned w) i.
-Definition trunc {n} m (w : bv n) : bv m := bv_zero_extend m w.
-Definition bv_eqb {n} (w1 w2 : bv n) : bool := Z.eqb (bv_unsigned w1) (bv_unsigned w2).
-(* The library puts the big end first. I want the little end first. *)
-Definition bv_concat n {n1 n2} (b1 : bv n1) (b2 : bv n2) : bv n := bv_concat n b2 b1.
+(*|
+1. Somehow, there doesn't seem to be a bit test function on bitvectors?
+|*)
 
-Definition add_with_carry {n} (c_in : bool) (w1 w2 : bv n) : bv n * bool :=
+Definition bit {n} i (w : bv n) : bool := Z.testbit (bv_unsigned w) i.
+
+(*|
+2. While zero-extension to a shorter word acts as truncation, that's really not intuitive when your code needs a truncation operation.
+|*)
+
+Definition trunc {n} m (w : bv n) : bv m := bv_zero_extend m w.
+
+(*|
+3. I need a boolean-valued equality test.
+|*)
+
+Definition bv_eqb {n} (w1 w2 : bv n) : bool :=
+    if decide (w1 = w2) then true else false.
+
+(*|
+4. The library's ``bv_concat`` takes the high word first. But I want to think in little-endian, so I need to swap that.
+|*)
+
+Definition bv_concat n {n1 n2} (b1 : bv n1) (b2 : bv n2) : bv n :=
+    bv_concat n b2 b1.
+
+(*|
+5. I need addition and subtraction operations that take and return carry bits.
+|*)
+
+Definition add_with_carry {n}
+    (c_in : bool) (w1 w2 : bv n) : bv n * bool :=
     let out :=
         bv_zero_extend (n + 1) (bool_to_bv 1 c_in) +
         (bv_zero_extend (n + 1) w1 + bv_zero_extend (n + 1) w2)
     in (trunc n out, bit (Z.of_N n) out).
-Definition sub_with_inverted_borrow {n} cin (w1 w2 : bv n) : bv n * bool :=
+Definition sub_with_inverted_borrow {n}
+    cin (w1 w2 : bv n) : bv n * bool :=
     add_with_carry cin w1 (bv_not w2).
 
+(*|
+-----------
+Atari State
+-----------
+
+The Atari 2600 uses a 6507 processor, which is basically a 6502 in a smaller package.
+
+The 6502 has four registers:
+* The accumulator, ``A``.
+* The index registers, ``X`` and ``Y``.
+* The stack pointer, ``SP``.
+|*)
+
 Inductive reg := X|Y|A|SP.
-Inductive flag := N|B|V|D|I|Z|C.
+
+Global Instance reg_eq_dec : EqDecision reg.
+Proof.
+    unfold EqDecision, Decision.
+    case; case; try (by left); by right.
+Defined.
 
 Definition reg_eqb (r1 r2 : reg) : bool :=
-    match (r1, r2) with
-    | (X,X) | (Y,Y) | (A,A) | (SP,SP) => true
-    | _ => false
-    end.
-Theorem reg_eqP {r1 r2} : reflect (r1 = r2) (reg_eqb r1 r2).
-Proof.
-    case r1; case r2; by constructor.
-Qed.
+    if decide (r1 = r2) then true else false.
 
-Definition flag_eqb (r1 r2 : flag) : bool :=
-    match (r1, r2) with
-    | (N,N) | (B,B) | (V,V) | (D,D) | (I,I) | (Z,Z) | (C,C) => true
-    | _ => false
-    end.
-Theorem flag_eqP {r1 r2} : reflect (r1 = r2) (flag_eqb r1 r2).
-Proof.
-    case r1; case r2; by constructor.
-Qed.
+(*|
+It also has seven boolean flags.
+|*)
 
+Inductive flag := N|B|V|D|I|Z|C.
+
+Global Instance flag_eq_dec : EqDecision flag.
+Proof.
+    unfold EqDecision, Decision.
+    case; case; try (by left); by right.
+Defined.
+
+Definition flag_eqb (f1 f2 : flag) : bool :=
+    if decide (f1 = f2) then true else false.
+
+(*|
+Finally, it has a sixteen-bit program counter.
+
+In addition to the processor, the Atari has 128 bytes of RAM.
+
+There are also a few other components, which handle things like hardware timers, I/O, and graphics.
+I take a very simple approach to modeling these: Don't!
+I make no assumptions at all about the result of reading from these chips, so I don't have to keep track of their state or behavior.
+
+With that in mind, the following structure models the state of the Atari.
+|*)
 
 Record state := {
+    (* processor *)
     Reg : reg -> bv 8;
     Flag : flag -> bool;
-    RAM : bv 7 -> bv 8;
     PC : bv 16;
+
+    (* memory *)
+    RAM : bv 7 -> bv 8;
 }.
+
+(*|
+----------------
+Reads and Writes
+----------------
+
+The Atari 2600's address space is memory-mapped as follows::
+
+    ___1 _xxx xxxx xxxx => ROM
+    ___0 ____ 0_xx xxxx => Television Interface Adapter
+    ___0 __1_ 1xxx xxxx => RAM
+    ___0 __0_ 1__x xxxx => Peripheral Interface Adapter
+
+(Technically, the Peripheral Interface Adapter contains the RAM. But I'm using the term to mean the part that isn't the RAM.)
+
+
+Let's implement this.
+|*)
+
+From theories Require Import rom.
+
+(*|
+``fetch s addr value`` is the statement, "If the Atari is in state ``s``, a read from ``addr`` *might* return ``value``.".
+
+In particular, when ``addr`` points to the TIA or PIA, ``fetch s addr value`` is simply ``True``.
+Since I don't model those components, I assume they can do anything they want.
+|*)
+
+Definition fetch (s : state) (addr : bv 16) (value : bv 8) : Prop :=
+    if bit 12 addr
+    then value = ROM (trunc 11 addr)
+    else if negb (bit 7 addr) || bit 9 addr
+    then True
+    else value = RAM s (trunc 7 addr).
+
+(*|
+If ``ram`` is the current state of the RAM, ``write addr value ram`` is the state after writing ``value`` to address ``addr``.
+
+Note that if you write to anything other than the RAM, nothing happens:
+
+* Writing to the TIA or PIA will change their state. But that state isn't modeled, so who cares?
+* If you write to the ROM...
+
+  Honestly, I can't find a clear answer for what happens.
+  But the ROM has no state to change, and all the other chips are deselected,
+  so the only reasonable option seems to be that nothing happens.
+
+.. coq::
+|*)
+
+Definition write (addr : bv 16) (value : bv 8)
+    (ram : bv 7 -> bv 8) : bv 7 -> bv 8 :=
+    if bit 12 addr
+    then ram
+    else if negb (bit 7 addr) || bit 9 addr
+    then ram
+    else fun addr' =>
+        if bv_eqb (trunc 7 addr) addr'
+        then value
+        else ram addr'.
+
+(*|
+-------
+Startup
+-------
+
+When the Atari is turned on, the interrupt-disable flag is turned on,
+and the program counter is set to the address stored at 0xfffc and 0xfffd.
+|*)
 
 Record initial (s : state) : Prop := {
     init_interrupt_disable : Flag s I;
-    pc_init : PC s = bv_concat 16 (ROM 0x7fc) (ROM 0x7fd)
+    pc_init : exists w1 w2,
+        fetch s 0xfffc w1 /\
+        fetch s 0xfffd w2 /\
+        PC s = bv_concat 16 w1 w2
 }.
 
-Definition fetch (s : state) (addr : bv 16) (value : bv 8) : Prop :=
-if bit 12 addr
-then value = ROM (trunc 11 addr)
-else if negb (bit 7 addr) || bit 9 addr
-(* TIA or PIA. I don't model these, so I assume they can return any value to the processor. *)
-then True
-else value = RAM s (trunc 7 addr).
+(*|
+--------------------
+Instruction Stepping
+--------------------
 
-Definition write (addr : bv 16) (value : bv 8) (ram : bv 7 -> bv 8) : bv 7 -> bv 8 :=
-if Z.testbit (bv_unsigned addr) 12
-then ram
-else if negb (Z.testbit (bv_unsigned addr) 7) || Z.testbit (bv_unsigned addr) 9
-then ram
-else fun addr' => if bv_eqb (trunc 7 addr) addr' then value else ram addr'.
+If the current state is ``s1``, is it possible that after one instruction, the state will be ``s2``?
+
+Recall that I am *overapproximating* the behavior of the Atari.
+So the specification takes the form a long list of restrictions.
+E.g. "If running instruction ``0xea`` can transform state ``s1`` into ``s2``,
+then we must have ``PC s2 = PC s1 + 1``, ``Reg s2 = Reg s1``, ``Flag s2 = Flag s1``, and ``RAM s2 = RAM s1``.".
+
+If you scroll to the bottom of this section, you'll find the record ``instruction``.
+This is that list. Everything above that is helper functions for defining the restrictions.
+|*)
 
 Section StepSpec.
 
 Context (s1 s2 : state).
 
-
-
-Definition setReg (r : reg) (value : bv 8) : reg -> bv 8 := fun r' =>
-    if reg_eqb r r' then value else Reg s1 r'.
+Definition setReg (r : reg) (value : bv 8) : reg -> bv 8 :=
+    fun r' => if reg_eqb r r' then value else Reg s1 r'.
 
 Definition setNZ (value : bv 8) : flag -> bool := fun f =>
     match f with
@@ -84,24 +234,29 @@ Definition setNZ (value : bv 8) : flag -> bool := fun f =>
     | _ => Flag s1 f
     end.
 
-Definition transfer_instruction r1 r2 :=
-    PC s2 = bv_add_Z (PC s1) 1 /\
+Definition transfer_instr r1 r2 :=
+    PC s2 = PC s1 `+Z` 1 /\
     Reg s2 = setReg r2 (Reg s1 r1) /\
     Flag s2 = setNZ (Reg s1 r1) /\
     RAM s2 = RAM s1.
 
-Definition flag_instruction (f : flag) (value : bool) : Prop :=
-    PC s2 = bv_add_Z (PC s1) 1 /\
+Definition flag_instr (f : flag) (value : bool) : Prop :=
+    PC s2 = PC s1 `+Z` 1 /\
     Reg s2 = Reg s1 /\
-    Flag s2 = (fun f' => if flag_eqb f f' then value else Flag s1 f') /\
+    (Flag s2 = fun f' => 
+        if flag_eqb f f'
+        then value
+        else Flag s1 f') /\
     RAM s2 = RAM s1.
 
-Definition branch_instruction (cond : state -> bool) : Prop :=
+Definition branch_instr (cond : state -> bool) : Prop :=
     exists dist,
-        fetch s1 (bv_add_Z (PC s1) 1) dist /\
+        fetch s1 (PC s1 `+Z` 1) dist /\
         (PC s2 =
-            let pc := bv_add_Z (PC s1) 2 in
-            if cond s1 then bv_add pc (bv_sign_extend 16 dist) else pc) /\
+            let pc := PC s1 `+Z` 2 in
+            if cond s1
+            then pc + bv_sign_extend 16 dist
+            else pc) /\
         Reg s2 = Reg s1 /\
         Flag s2 = Flag s1 /\
         RAM s2 = RAM s1.
@@ -109,72 +264,73 @@ Definition branch_instruction (cond : state -> bool) : Prop :=
 Definition mem_addressing_mode := state -> bv 16 -> Prop.
 Definition absolute : mem_addressing_mode :=
     fun s addr => exists w1 w2,
-        fetch s (bv_add_Z (PC s) 1) w1 /\
-        fetch s (bv_add_Z (PC s) 2) w2 /\
+        fetch s (PC s `+Z` 1) w1 /\
+        fetch s (PC s `+Z` 2) w2 /\
         addr = bv_concat 16 w1 w2.
 Definition absolute_x : mem_addressing_mode :=
     fun s addr => exists w1 w2,
-        fetch s (bv_add_Z (PC s) 1) w1 /\
-        fetch s (bv_add_Z (PC s) 2) w2 /\
-        addr = bv_add (bv_concat 16 w1 w2) (bv_zero_extend 16 (Reg s X)).
+        fetch s (PC s `+Z` 1) w1 /\
+        fetch s (PC s `+Z` 2) w2 /\
+        addr = bv_concat 16 w1 w2 + bv_zero_extend 16 (Reg s X).
 Definition absolute_y : mem_addressing_mode :=
     fun s addr => exists w1 w2,
-        fetch s (bv_add_Z (PC s) 1) w1 /\
-        fetch s (bv_add_Z (PC s) 2) w2 /\
-        addr = bv_add (bv_concat 16 w1 w2) (bv_zero_extend 16 (Reg s Y)).
+        fetch s (PC s `+Z` 1) w1 /\
+        fetch s (PC s `+Z` 2) w2 /\
+        addr = bv_concat 16 w1 w2 + bv_zero_extend 16 (Reg s Y).
 Definition zero_page : mem_addressing_mode :=
     fun s addr => exists w,
-        fetch s (bv_add_Z (PC s) 1) w /\
+        fetch s (PC s `+Z` 1) w /\
         addr = bv_zero_extend 16 w.
 Definition zero_page_x : mem_addressing_mode :=
     fun s addr => exists w,
-        fetch s (bv_add_Z (PC s) 1) w /\
-        addr = bv_zero_extend 16 (bv_add w (Reg s X)).
+        fetch s (PC s `+Z` 1) w /\
+        addr = bv_zero_extend 16 (w + Reg s X).
 Definition zero_page_y : mem_addressing_mode :=
     fun s addr => exists w,
-        fetch s (bv_add_Z (PC s) 1) w /\
-        addr = bv_zero_extend 16 (bv_add w (Reg s Y)).
+        fetch s (PC s `+Z` 1) w /\
+        addr = bv_zero_extend 16 (w + Reg s Y).
 Definition indirect_x : mem_addressing_mode :=
     fun s addr => exists w w1 w2,
-        fetch s (bv_add_Z (PC s) 1) w /\
-        let indir := bv_add w (Reg s X) in
+        fetch s (PC s `+Z` 1) w /\
+        let indir := w + Reg s X in
         fetch s (bv_zero_extend 16 indir) w1 /\
-        fetch s (bv_zero_extend 16 (bv_add_Z indir 1)) w2 /\
+        fetch s (bv_zero_extend 16 (indir `+Z` 1)) w2 /\
         addr = bv_concat 16 w1 w2.
 Definition indirect_y : mem_addressing_mode :=
     fun s addr => exists indir w1 w2,
-        fetch s (bv_add_Z (PC s) 1) indir /\
+        fetch s (PC s `+Z` 1) indir /\
         fetch s (bv_zero_extend 16 indir) w1 /\
-        fetch s (bv_zero_extend 16 (bv_add_Z indir 1)) w2 /\
-        addr = bv_add (bv_concat 16 w1 w2) (bv_zero_extend 16 (Reg s Y)).
+        fetch s (bv_zero_extend 16 (indir `+Z` 1)) w2 /\
+        addr = bv_concat 16 w1 w2 + bv_zero_extend 16 (Reg s Y).
 (* This isn't traditionally treated as a *memory* addressing mode.
-But in a sense, it is. It accesses the memory immediately following the opcode! *)
+    But in a sense, it is.
+    It accesses the memory immediately following the opcode! *)
 Definition immediate : mem_addressing_mode :=
-    fun s addr => addr = bv_add_Z (PC s) 1.
+    fun s addr => addr = PC s `+Z` 1.
 
-Definition store_instruction register mode mode_len :=
+Definition store_instr register mode mode_len :=
     exists addr,
         mode s1 addr /\
-        PC s2 = bv_add_Z (PC s1) mode_len /\
+        PC s2 = PC s1 `+Z` mode_len /\
         Reg s2 = Reg s1 /\
         Flag s2 = Flag s1 /\
         RAM s2 = write addr (Reg s1 register) (RAM s1).
 
-Definition load_instruction register mode mode_len :=
+Definition load_instr register mode mode_len :=
     exists addr w,
         mode s1 addr /\
         fetch s1 addr w /\
-        PC s2 = bv_add_Z (PC s1) mode_len /\
+        PC s2 = PC s1 `+Z` mode_len /\
         Reg s2 = setReg register w /\
         Flag s2 = setNZ w /\
         RAM s2 = RAM s1.
 
-Definition logic_instruction operation mode mode_len :=
+Definition logic_instr operation mode mode_len :=
     exists addr w,
         mode s1 addr /\
         fetch s1 addr w /\
         let w := operation (Reg s1 A) w in
-        PC s2 = bv_add_Z (PC s1) mode_len /\
+        PC s2 = PC s1 `+Z` mode_len /\
         Reg s2 = setReg A w /\
         Flag s2 = setNZ w /\
         RAM s2 = RAM s1.
@@ -184,7 +340,7 @@ Definition BIT_mode mode mode_len :=
         mode s1 addr /\
         fetch s1 addr w /\
         let w := bv_and (Reg s1 A) w in
-        PC s2 = bv_add_Z (PC s1) mode_len /\
+        PC s2 = PC s1 `+Z` mode_len /\
         Reg s2 = Reg s1 /\
         Flag s2 = (fun f =>
             match f with
@@ -196,8 +352,8 @@ Definition BIT_mode mode mode_len :=
         RAM s2 = RAM s1.
 
 Definition INC_reg r :=
-    let w := bv_add_Z (Reg s1 r) 1 in
-    PC s2 = bv_add_Z (PC s1) 1 /\
+    let w := Reg s1 r `+Z` 1 in
+    PC s2 = PC s1 `+Z` 1 /\
     Reg s2 = setReg r w /\
     Flag s2 = setNZ w /\
     RAM s2 = RAM s1.
@@ -205,14 +361,14 @@ Definition INC_mode mode mode_len :=
     exists addr w,
         mode s1 addr /\
         fetch s1 addr w /\
-        let w := bv_add_Z w 1 in
-        PC s2 = bv_add_Z (PC s1) mode_len /\
+        let w := w `+Z` 1 in
+        PC s2 = PC s1 `+Z` mode_len /\
         Reg s2 = Reg s1 /\
         Flag s2 = setNZ w /\
         RAM s2 = write addr w (RAM s1).
 Definition DEC_reg r :=
-    let w := bv_sub_Z (Reg s1 r) 1 in
-    PC s2 = bv_add_Z (PC s1) 1 /\
+    let w := Reg s1 r `-Z` 1 in
+    PC s2 = PC s1 `+Z` 1 /\
     Reg s2 = setReg r w /\
     Flag s2 = setNZ w /\
     RAM s2 = RAM s1.
@@ -221,18 +377,19 @@ Definition DEC_mode mode mode_len :=
         mode s1 addr /\
         fetch s1 addr w /\
         let w := bv_sub_Z w 1 in
-        PC s2 = bv_add_Z (PC s1) mode_len /\
+        PC s2 = PC s1 `+Z` mode_len /\
         Reg s2 = Reg s1 /\
         Flag s2 = setNZ w /\
         RAM s2 = write addr w (RAM s1).
 
 
-Definition shift_instruction_A (shift_spec : bv 8 -> bool -> bv 8 -> bool -> Prop) :=
+Definition shift_instr_A
+    (shift_spec : bv 8 -> bool -> bv 8 -> bool -> Prop) :=
     exists cout (w : bv 8),
         shift_spec
             (Reg s1 A) (Flag s1 C)
             w cout /\
-        PC s2 = bv_add_Z (PC s1) 1 /\
+        PC s2 = PC s1 `+Z` 1 /\
         Reg s2 = setReg A w /\
         Flag s2 = (fun f =>
             match f with
@@ -242,7 +399,7 @@ Definition shift_instruction_A (shift_spec : bv 8 -> bool -> bv 8 -> bool -> Pro
             | _ => Flag s1 f
             end) /\
         RAM s2 = RAM s1.
-Definition shift_instruction_mode
+Definition shift_instr_mode
     (shift_spec : bv 8 -> bool -> bv 8 -> bool -> Prop) mode mode_len :=
     exists addr w_in cout (w_out : bv 8),
         mode s1 addr /\
@@ -250,7 +407,7 @@ Definition shift_instruction_mode
         shift_spec
             w_in (Flag s1 C)
             w_out cout /\
-        PC s2 = bv_add_Z (PC s1) mode_len /\
+        PC s2 = PC s1 `+Z` mode_len /\
         Reg s2 = Reg s1 /\
         Flag s2 = (fun f =>
             match f with
@@ -278,8 +435,10 @@ Definition CMP_mode register mode mode_len :=
     exists addr w,
         mode s1 addr /\
         fetch s1 addr w /\
-        let: (w, c) := sub_with_inverted_borrow true (Reg s1 register) w in
-        PC s2 = bv_add_Z (PC s1) mode_len /\
+        let: (w, c) :=
+            sub_with_inverted_borrow true (Reg s1 register) w
+        in
+        PC s2 = PC s1 `+Z` mode_len /\
         Reg s2 = Reg s1 /\
         Flag s2 = (fun f =>
             match f with
@@ -297,10 +456,13 @@ Definition is_bcd (w : bv 8) (n : BinNums.Z) : Prop :=
         bv_unsigned w2 <? 10 /\
         n = bv_unsigned w1 * 10 + bv_unsigned w2)%Z.
 
-Definition ADC_decimal_relation (c_in : bool) (w1 w2 w : bv 8) (c_out : bool) : Prop :=
+Definition ADC_decimal_relation
+    (c_in : bool) (w1 w2 w : bv 8) (c_out : bool) : Prop :=
     forall n1 n2, is_bcd w1 n1 -> is_bcd w2 n2 ->
     exists n, is_bcd w n /\
-    (n + (if c_out then 100 else 0) = (if c_in then 1 else 0) + n1 + n2)%Z.
+    ( n + (if c_out then 100 else 0)
+    = (if c_in then 1 else 0) + n1 + n2
+    )%Z.
 
 Definition ADC_mode mode mode_len :=
     if Flag s1 D
@@ -308,7 +470,7 @@ Definition ADC_mode mode mode_len :=
         mode s1 addr /\
         fetch s1 addr w_in /\
         ADC_decimal_relation (Flag s1 C) (Reg s1 A) w_in w_out c_out /\
-        PC s2 = bv_add_Z (PC s1) mode_len /\
+        PC s2 = PC s1 `+Z` mode_len /\
         Reg s2 = setReg A w_out /\
         Flag s2 = (fun f =>
             match f with
@@ -322,8 +484,10 @@ Definition ADC_mode mode mode_len :=
     else exists addr w_in,
         mode s1 addr /\
         fetch s1 addr w_in /\
-        let: (w_out, c) := add_with_carry (Flag s1 C) (Reg s1 A) w_in in
-        PC s2 = bv_add_Z (PC s1) mode_len /\
+        let:
+            (w_out, c) := add_with_carry (Flag s1 C) (Reg s1 A) w_in
+        in
+        PC s2 = PC s1 `+Z` mode_len /\
         Reg s2 = setReg A w_out /\
         Flag s2 = (fun f =>
             match f with
@@ -337,10 +501,12 @@ Definition ADC_mode mode mode_len :=
             end) /\
         RAM s2 = RAM s1.
 
-Definition SBC_decimal_relation (c_in : bool) (w1 w2 w : bv 8) (c_out : bool) : Prop :=
+Definition SBC_decimal_relation
+    (c_in : bool) (w1 w2 w : bv 8) (c_out : bool) : Prop :=
     forall n1 n2, is_bcd w1 n1 -> is_bcd w2 n2 ->
     exists n, is_bcd w n /\
-    (n + (if c_out then 0 else 100) + n2 + (if c_in then 0 else 1) = n1)%Z.
+    ( n + (if c_out then 0 else 100) + n2 + (if c_in then 0 else 1)
+    = n1)%Z.
 
 Definition SBC_mode mode mode_len :=
     if Flag s1 D
@@ -348,7 +514,7 @@ Definition SBC_mode mode mode_len :=
         mode s1 addr /\
         fetch s1 addr w_in /\
         SBC_decimal_relation (Flag s1 C) (Reg s1 A) w_in w_out c_out /\
-        PC s2 = bv_add_Z (PC s1) mode_len /\
+        PC s2 = PC s1 `+Z` mode_len /\
         Reg s2 = setReg A w_out /\
         Flag s2 = (fun f =>
             match f with
@@ -362,8 +528,10 @@ Definition SBC_mode mode mode_len :=
     else exists addr w_in,
         mode s1 addr /\
         fetch s1 addr w_in /\
-        let: (w_out, c) := sub_with_inverted_borrow (Flag s1 C) (Reg s1 A) w_in in
-        PC s2 = bv_add_Z (PC s1) mode_len /\
+        let: (w_out, c) :=
+            sub_with_inverted_borrow (Flag s1 C) (Reg s1 A) w_in
+        in
+        PC s2 = PC s1 `+Z` mode_len /\
         Reg s2 = setReg A w_out /\
         Flag s2 = (fun f =>
             match f with
@@ -379,97 +547,105 @@ Definition SBC_mode mode mode_len :=
 
 
 Record instruction (op : bv 8) : Prop := {
-    NOP : op = 0xea -> PC s2 = bv_add_Z (PC s1) 1 /\ Reg s2 = Reg s1 /\ Flag s2 = Flag s1 /\ RAM s2 = RAM s1;
-
-    TXS : op = 0x9a -> PC s2 = bv_add_Z (PC s1) 1 /\ Reg s2 = setReg SP (Reg s1 X) /\ Flag s2 = Flag s1 /\ RAM s2 = RAM s1;
-    TSX : op = 0xba -> transfer_instruction SP X;
-    TAX : op = 0xaa -> transfer_instruction A X;
-    TXA : op = 0x8a -> transfer_instruction X A;
-    TAY : op = 0xa8 -> transfer_instruction A Y;
-    TYA : op = 0x98 -> transfer_instruction Y A;
-
-    CLC : op = 0x18 -> flag_instruction C false;
-    SEC : op = 0x38 -> flag_instruction C true;
-    CLI : op = 0x58 -> flag_instruction I false;
-    SEI : op = 0x78 -> flag_instruction I true;
-    CLV : op = 0xb8 -> flag_instruction V false;
-    CLD : op = 0xd8 -> flag_instruction D false;
-    SED : op = 0xf8 -> flag_instruction D true;
-
-    RTS : op = 0x60 -> exists w1 w2,
-        fetch s1 (bv_zero_extend 16 (bv_add_Z (Reg s1 SP) 1)) w1 /\
-        fetch s2 (bv_zero_extend 16 (bv_add_Z (Reg s1 SP) 2)) w2 /\
-        PC s2 = bv_add_Z (bv_concat 16 w1 w2) 1 /\
+    NOP : op = 0xea ->
+        PC s2 = PC s1 `+Z` 1 /\
         Reg s2 = Reg s1 /\
         Flag s2 = Flag s1 /\
         RAM s2 = RAM s1;
 
-    BPL : op = 0x10 -> branch_instruction (fun s => negb (Flag s N));
-    BMI : op = 0x30 -> branch_instruction (fun s =>      (Flag s N));
-    BVC : op = 0x50 -> branch_instruction (fun s => negb (Flag s V));
-    BVS : op = 0x70 -> branch_instruction (fun s =>      (Flag s V));
-    BCC : op = 0x90 -> branch_instruction (fun s => negb (Flag s N));
-    BCS : op = 0xb0 -> branch_instruction (fun s =>      (Flag s N));
-    BNE : op = 0xd0 -> branch_instruction (fun s => negb (Flag s Z));
-    BEQ : op = 0xf0 -> branch_instruction (fun s =>      (Flag s Z));
+    TXS : op = 0x9a ->
+        PC s2 = PC s1 `+Z` 1 /\
+        Reg s2 = setReg SP (Reg s1 X) /\
+        Flag s2 = Flag s1 /\
+        RAM s2 = RAM s1;
+    TSX : op = 0xba -> transfer_instr SP X;
+    TAX : op = 0xaa -> transfer_instr A X;
+    TXA : op = 0x8a -> transfer_instr X A;
+    TAY : op = 0xa8 -> transfer_instr A Y;
+    TYA : op = 0x98 -> transfer_instr Y A;
 
-    STA_absolute   : op = 0x8d -> store_instruction A absolute 3;
-    STX_absolute   : op = 0x8e -> store_instruction X absolute 3;
-    STY_absolute   : op = 0x8c -> store_instruction Y absolute 3;
-    STA_absolute_x : op = 0x9d -> store_instruction A absolute_x 3;
-    STA_absolute_y : op = 0x99 -> store_instruction A absolute_y 3;
-    STA_zero_page  : op = 0x85 -> store_instruction A zero_page 2;
-    STX_zero_page  : op = 0x86 -> store_instruction X zero_page 2;
-    STY_zero_page  : op = 0x84 -> store_instruction Y zero_page 2;
-    STA_zero_page_x: op = 0x95 -> store_instruction A zero_page_x 2;
-    STX_zero_page_y: op = 0x96 -> store_instruction X zero_page_y 2;
-    STY_zero_page_x: op = 0x94 -> store_instruction Y zero_page_x 2;
-    STA_indirect_x : op = 0x81 -> store_instruction A indirect_x 2;
-    STA_indirect_y : op = 0x91 -> store_instruction A indirect_y 2;
+    CLC : op = 0x18 -> flag_instr C false;
+    SEC : op = 0x38 -> flag_instr C true;
+    CLI : op = 0x58 -> flag_instr I false;
+    SEI : op = 0x78 -> flag_instr I true;
+    CLV : op = 0xb8 -> flag_instr V false;
+    CLD : op = 0xd8 -> flag_instr D false;
+    SED : op = 0xf8 -> flag_instr D true;
 
-    LDA_absolute   : op = 0xad -> load_instruction A absolute 3;
-    LDX_absolute   : op = 0xae -> load_instruction X absolute 3;
-    LDY_absolute   : op = 0xac -> load_instruction Y absolute 3;
-    LDA_absolute_x : op = 0xbd -> load_instruction A absolute_x 3;
-    LDA_absolute_y : op = 0xb9 -> load_instruction A absolute_y 3;
-    LDX_absolute_y : op = 0xbe -> load_instruction X absolute_y 3;
-    LDY_absolute_x : op = 0xbc -> load_instruction Y absolute_x 3;
-    LDA_immediate  : op = 0xa9 -> load_instruction A immediate 2;
-    LDX_immediate  : op = 0xa2 -> load_instruction X immediate 2;
-    LDY_immediate  : op = 0xa0 -> load_instruction Y immediate 2;
-    LDA_zero_page  : op = 0xa5 -> load_instruction A zero_page 2;
-    LDX_zero_page  : op = 0xa6 -> load_instruction X zero_page 2;
-    LDY_zero_page  : op = 0xa4 -> load_instruction Y zero_page 2;
-    LDA_zero_page_x: op = 0xb5 -> load_instruction A zero_page_x 2;
-    LDX_zero_page_y: op = 0xb6 -> load_instruction X zero_page_y 2;
-    LDY_zero_page_x: op = 0xb4 -> load_instruction Y zero_page_x 2;
-    LDA_indirect_x : op = 0xa1 -> load_instruction A indirect_x 2;
-    LDA_indirect_y : op = 0xb1 -> load_instruction A indirect_y 2;
-    
-    ORA_indirect_x : op = 0x01 -> logic_instruction bv_or  indirect_x 2;
-    ORA_zero_page  : op = 0x05 -> logic_instruction bv_or  zero_page  2;
-    ORA_immediate  : op = 0x09 -> logic_instruction bv_or  immediate  2;
-    ORA_absolute   : op = 0x0d -> logic_instruction bv_or  absolute   3;
-    ORA_indirect_y : op = 0x11 -> logic_instruction bv_or  indirect_y 2;
-    ORA_zero_page_x: op = 0x15 -> logic_instruction bv_or  zero_page_x 2;
-    ORA_absolute_y : op = 0x19 -> logic_instruction bv_or  absolute_y 3;
-    ORA_absolute_x : op = 0x1d -> logic_instruction bv_or  absolute_x 3;
-    AND_indirect_x : op = 0x21 -> logic_instruction bv_and indirect_x 2;
-    AND_zero_page  : op = 0x25 -> logic_instruction bv_and zero_page  2;
-    AND_immediate  : op = 0x29 -> logic_instruction bv_and immediate  2;
-    AND_absolute   : op = 0x2d -> logic_instruction bv_and absolute   3;
-    AND_indirect_y : op = 0x31 -> logic_instruction bv_and indirect_y 2;
-    AND_zero_page_x: op = 0x35 -> logic_instruction bv_and zero_page_x 2;
-    AND_absolute_y : op = 0x39 -> logic_instruction bv_and absolute_y 3;
-    AND_absolute_x : op = 0x3d -> logic_instruction bv_and absolute_x 3;
-    EOR_indirect_x : op = 0x41 -> logic_instruction bv_xor indirect_x 2;
-    EOR_zero_page  : op = 0x45 -> logic_instruction bv_xor zero_page  2;
-    EOR_immediate  : op = 0x49 -> logic_instruction bv_xor immediate  2;
-    EOR_absolute   : op = 0x4d -> logic_instruction bv_xor absolute   3;
-    EOR_indirect_y : op = 0x51 -> logic_instruction bv_xor indirect_y 2;
-    EOR_zero_page_x: op = 0x55 -> logic_instruction bv_xor zero_page_x 2;
-    EOR_absolute_y : op = 0x59 -> logic_instruction bv_xor absolute_y 3;
-    EOR_absolute_x : op = 0x5d -> logic_instruction bv_xor absolute_x 3;
+    RTS : op = 0x60 -> exists w1 w2,
+        fetch s1 (bv_zero_extend 16 (Reg s1 SP `+Z` 1)) w1 /\
+        fetch s2 (bv_zero_extend 16 (Reg s1 SP `+Z` 2)) w2 /\
+        PC s2 = bv_concat 16 w1 w2 `+Z` 1 /\
+        Reg s2 = Reg s1 /\
+        Flag s2 = Flag s1 /\
+        RAM s2 = RAM s1;
+
+    BPL : op = 0x10 -> branch_instr (fun s => negb (Flag s N));
+    BMI : op = 0x30 -> branch_instr (fun s =>      (Flag s N));
+    BVC : op = 0x50 -> branch_instr (fun s => negb (Flag s V));
+    BVS : op = 0x70 -> branch_instr (fun s =>      (Flag s V));
+    BCC : op = 0x90 -> branch_instr (fun s => negb (Flag s N));
+    BCS : op = 0xb0 -> branch_instr (fun s =>      (Flag s N));
+    BNE : op = 0xd0 -> branch_instr (fun s => negb (Flag s Z));
+    BEQ : op = 0xf0 -> branch_instr (fun s =>      (Flag s Z));
+
+    STA_absolute   : op = 0x8d -> store_instr A absolute 3;
+    STX_absolute   : op = 0x8e -> store_instr X absolute 3;
+    STY_absolute   : op = 0x8c -> store_instr Y absolute 3;
+    STA_absolute_x : op = 0x9d -> store_instr A absolute_x 3;
+    STA_absolute_y : op = 0x99 -> store_instr A absolute_y 3;
+    STA_zero_page  : op = 0x85 -> store_instr A zero_page 2;
+    STX_zero_page  : op = 0x86 -> store_instr X zero_page 2;
+    STY_zero_page  : op = 0x84 -> store_instr Y zero_page 2;
+    STA_zero_page_x: op = 0x95 -> store_instr A zero_page_x 2;
+    STX_zero_page_y: op = 0x96 -> store_instr X zero_page_y 2;
+    STY_zero_page_x: op = 0x94 -> store_instr Y zero_page_x 2;
+    STA_indirect_x : op = 0x81 -> store_instr A indirect_x 2;
+    STA_indirect_y : op = 0x91 -> store_instr A indirect_y 2;
+
+    LDA_absolute   : op = 0xad -> load_instr A absolute 3;
+    LDX_absolute   : op = 0xae -> load_instr X absolute 3;
+    LDY_absolute   : op = 0xac -> load_instr Y absolute 3;
+    LDA_absolute_x : op = 0xbd -> load_instr A absolute_x 3;
+    LDA_absolute_y : op = 0xb9 -> load_instr A absolute_y 3;
+    LDX_absolute_y : op = 0xbe -> load_instr X absolute_y 3;
+    LDY_absolute_x : op = 0xbc -> load_instr Y absolute_x 3;
+    LDA_immediate  : op = 0xa9 -> load_instr A immediate 2;
+    LDX_immediate  : op = 0xa2 -> load_instr X immediate 2;
+    LDY_immediate  : op = 0xa0 -> load_instr Y immediate 2;
+    LDA_zero_page  : op = 0xa5 -> load_instr A zero_page 2;
+    LDX_zero_page  : op = 0xa6 -> load_instr X zero_page 2;
+    LDY_zero_page  : op = 0xa4 -> load_instr Y zero_page 2;
+    LDA_zero_page_x: op = 0xb5 -> load_instr A zero_page_x 2;
+    LDX_zero_page_y: op = 0xb6 -> load_instr X zero_page_y 2;
+    LDY_zero_page_x: op = 0xb4 -> load_instr Y zero_page_x 2;
+    LDA_indirect_x : op = 0xa1 -> load_instr A indirect_x 2;
+    LDA_indirect_y : op = 0xb1 -> load_instr A indirect_y 2;
+
+    ORA_indirect_x : op = 0x01 -> logic_instr bv_or  indirect_x 2;
+    ORA_zero_page  : op = 0x05 -> logic_instr bv_or  zero_page  2;
+    ORA_immediate  : op = 0x09 -> logic_instr bv_or  immediate  2;
+    ORA_absolute   : op = 0x0d -> logic_instr bv_or  absolute   3;
+    ORA_indirect_y : op = 0x11 -> logic_instr bv_or  indirect_y 2;
+    ORA_zero_page_x: op = 0x15 -> logic_instr bv_or  zero_page_x 2;
+    ORA_absolute_y : op = 0x19 -> logic_instr bv_or  absolute_y 3;
+    ORA_absolute_x : op = 0x1d -> logic_instr bv_or  absolute_x 3;
+    AND_indirect_x : op = 0x21 -> logic_instr bv_and indirect_x 2;
+    AND_zero_page  : op = 0x25 -> logic_instr bv_and zero_page  2;
+    AND_immediate  : op = 0x29 -> logic_instr bv_and immediate  2;
+    AND_absolute   : op = 0x2d -> logic_instr bv_and absolute   3;
+    AND_indirect_y : op = 0x31 -> logic_instr bv_and indirect_y 2;
+    AND_zero_page_x: op = 0x35 -> logic_instr bv_and zero_page_x 2;
+    AND_absolute_y : op = 0x39 -> logic_instr bv_and absolute_y 3;
+    AND_absolute_x : op = 0x3d -> logic_instr bv_and absolute_x 3;
+    EOR_indirect_x : op = 0x41 -> logic_instr bv_xor indirect_x 2;
+    EOR_zero_page  : op = 0x45 -> logic_instr bv_xor zero_page  2;
+    EOR_immediate  : op = 0x49 -> logic_instr bv_xor immediate  2;
+    EOR_absolute   : op = 0x4d -> logic_instr bv_xor absolute   3;
+    EOR_indirect_y : op = 0x51 -> logic_instr bv_xor indirect_y 2;
+    EOR_zero_page_x: op = 0x55 -> logic_instr bv_xor zero_page_x 2;
+    EOR_absolute_y : op = 0x59 -> logic_instr bv_xor absolute_y 3;
+    EOR_absolute_x : op = 0x5d -> logic_instr bv_xor absolute_x 3;
 
     BIT_absolute   : op = 0x2c -> BIT_mode absolute  3;
     BIT_zero_page  : op = 0x24 -> BIT_mode zero_page 2;
@@ -479,7 +655,7 @@ Record instruction (op : bv 8) : Prop := {
     INY : op = 0xc8 -> INC_reg Y;
     DEX : op = 0xca -> DEC_reg X;
     DEY : op = 0x88 -> DEC_reg Y;
-    
+
     INC_absolute   : op = 0xee -> INC_mode absolute 3;
     INC_absolute_x : op = 0xfe -> INC_mode absolute_x 3;
     INC_zero_page  : op = 0xe6 -> INC_mode zero_page 2;
@@ -489,27 +665,27 @@ Record instruction (op : bv 8) : Prop := {
     DEC_zero_page  : op = 0xc6 -> DEC_mode zero_page 2;
     DEC_zero_page_x: op = 0xd6 -> DEC_mode zero_page_x 2;
 
-    ASL_A          : op = 0x0a -> shift_instruction_A ASL_spec;
-    ROL_A          : op = 0x2a -> shift_instruction_A ROL_spec;
-    LSR_A          : op = 0x4a -> shift_instruction_A LSR_spec;
-    ROR_A          : op = 0x6a -> shift_instruction_A ROR_spec;
-    ASL_absolute   : op = 0x0e -> shift_instruction_mode ASL_spec absolute 3;
-    ROL_absolute   : op = 0x2e -> shift_instruction_mode ROL_spec absolute 3;
-    LSR_absolute   : op = 0x4e -> shift_instruction_mode LSR_spec absolute 3;
-    ROR_absolute   : op = 0x6e -> shift_instruction_mode ROR_spec absolute 3;
-    ASL_absolute_x : op = 0x1e -> shift_instruction_mode ASL_spec absolute_x 3;
-    ROL_absolute_x : op = 0x3e -> shift_instruction_mode ROL_spec absolute_x 3;
-    LSR_absolute_x : op = 0x5e -> shift_instruction_mode LSR_spec absolute_x 3;
-    ROR_absolute_x : op = 0x7e -> shift_instruction_mode ROR_spec absolute_x 3;
-    ASL_zero_page  : op = 0x06 -> shift_instruction_mode ASL_spec zero_page 2;
-    ROL_zero_page  : op = 0x26 -> shift_instruction_mode ROL_spec zero_page 2;
-    LSR_zero_page  : op = 0x46 -> shift_instruction_mode LSR_spec zero_page 2;
-    ROR_zero_page  : op = 0x66 -> shift_instruction_mode ROR_spec zero_page 2;
-    ASL_zero_page_x: op = 0x16 -> shift_instruction_mode ASL_spec zero_page_x 2;
-    ROL_zero_page_x: op = 0x36 -> shift_instruction_mode ROL_spec zero_page_x 2;
-    LSR_zero_page_x: op = 0x56 -> shift_instruction_mode LSR_spec zero_page_x 2;
-    ROR_zero_page_x: op = 0x76 -> shift_instruction_mode ROR_spec zero_page_x 2;
-    
+    ASL_A          : op = 0x0a->shift_instr_A ASL_spec;
+    ROL_A          : op = 0x2a->shift_instr_A ROL_spec;
+    LSR_A          : op = 0x4a->shift_instr_A LSR_spec;
+    ROR_A          : op = 0x6a->shift_instr_A ROR_spec;
+    ASL_absolute   : op = 0x0e->shift_instr_mode ASL_spec absolute 3;
+    ROL_absolute   : op = 0x2e->shift_instr_mode ROL_spec absolute 3;
+    LSR_absolute   : op = 0x4e->shift_instr_mode LSR_spec absolute 3;
+    ROR_absolute   : op = 0x6e->shift_instr_mode ROR_spec absolute 3;
+    ASL_absolute_x : op = 0x1e->shift_instr_mode ASL_spec absolute_x 3;
+    ROL_absolute_x : op = 0x3e->shift_instr_mode ROL_spec absolute_x 3;
+    LSR_absolute_x : op = 0x5e->shift_instr_mode LSR_spec absolute_x 3;
+    ROR_absolute_x : op = 0x7e->shift_instr_mode ROR_spec absolute_x 3;
+    ASL_zero_page  : op = 0x06->shift_instr_mode ASL_spec zero_page 2;
+    ROL_zero_page  : op = 0x26->shift_instr_mode ROL_spec zero_page 2;
+    LSR_zero_page  : op = 0x46->shift_instr_mode LSR_spec zero_page 2;
+    ROR_zero_page  : op = 0x66->shift_instr_mode ROR_spec zero_page 2;
+    ASL_zero_page_x: op = 0x16->shift_instr_mode ASL_spec zero_page_x 2;
+    ROL_zero_page_x: op = 0x36->shift_instr_mode ROL_spec zero_page_x 2;
+    LSR_zero_page_x: op = 0x56->shift_instr_mode LSR_spec zero_page_x 2;
+    ROR_zero_page_x: op = 0x76->shift_instr_mode ROR_spec zero_page_x 2;
+
     CMP_absolute   : op = 0xcd -> CMP_mode A absolute    3;
     CPX_absolute   : op = 0xec -> CMP_mode X absolute    3;
     CPY_absolute   : op = 0xcc -> CMP_mode Y absolute    3;
@@ -524,7 +700,7 @@ Record instruction (op : bv 8) : Prop := {
     CMP_zero_page_x: op = 0xd5 -> CMP_mode A zero_page_x 2;
     CMP_indirect_x : op = 0xc1 -> CMP_mode A indirect_x  2;
     CMP_indirect_y : op = 0xd1 -> CMP_mode A indirect_y  2;
-    
+
     ADC_absolute   : op = 0x6d -> ADC_mode absolute    3;
     ADC_absolute_x : op = 0x7d -> ADC_mode absolute_x  3;
     ADC_absolute_y : op = 0x79 -> ADC_mode absolute_y  3;
@@ -543,8 +719,13 @@ Record instruction (op : bv 8) : Prop := {
     SBC_indirect_y : op = 0xf1 -> SBC_mode indirect_y  2;
 
     JMP : op = 0x4c -> exists addr,
-        absolute s1 addr /\ PC s2 = addr /\ Reg s2 = Reg s1 /\ Flag s2 = Flag s1 /\ RAM s2 = RAM s1;
-    (* Note: If I were to specify JMP_indirect, I'd have to account for the hardware bug. *)
+        absolute s1 addr /\
+        PC s2 = addr /\
+        Reg s2 = Reg s1 /\
+        Flag s2 = Flag s1 /\
+        RAM s2 = RAM s1;
+    (* Note: If I were to specify JMP_indirect,
+        I'd have to account for the hardware bug. *)
 
     JSR : op = 0x20 -> exists addr,
         absolute s1 addr /\
@@ -553,50 +734,85 @@ Record instruction (op : bv 8) : Prop := {
         Flag s2 = Flag s1 /\
         RAM s2 =
             let pc := bv_sub_Z (PC s1) 1 in
-            write (bv_zero_extend 16 (bv_sub_Z (Reg s1 SP) 1)) (bv_extract 0 8 pc)
-                (write (bv_zero_extend 16 (Reg s1 SP)) (bv_extract 0 8 pc)
+            write
+                (bv_zero_extend 16 (bv_sub_Z (Reg s1 SP) 1))
+                (bv_extract 0 8 pc)
+                (write
+                    (bv_zero_extend 16 (Reg s1 SP))
+                    (bv_extract 0 8 pc)
                     (RAM s1));
 }.
 
-Definition step : Prop := exists opcode, fetch s1 (PC s1) opcode /\ instruction opcode.
-
+Definition step : Prop :=
+    exists opcode, fetch s1 (PC s1) opcode /\ instruction opcode.
 
 End StepSpec.
 
+(*|
+This completes the specification of the Atari.
 
+----
+Goal
+----
 
+Ultimately, we want to prove that Dragster cannot be beaten in less than 5.57 seconds.
+Here, I simply *state* the claim.
 
+What does it mean to win Dragster?
 
+The best I can figure out is that Dragster has been won if the branch at address 0xF39E is taken.
+I was hoping there'd be a variable that clearly says "You have won!", but I couldn't find one.
+|*)
+
+Definition someone_has_won (s : state) :=
+    trunc 11 (PC s) = 0x39e /\ ~~ Flag s Z.
+
+(*|
+But we need to know *who* has won, so we can check the right player's timer.
+
+The active player is stored at RAM location 0x0f.
+|*)
 
 Inductive Player := P0 | P1.
 
 Definition player_active (s : state) (p : Player) :=
     RAM s 0x0f = match p with P0 => 0x00 | P1 => 0x01 end.
 
-(*
-What does it mean to win Dragster?
+Definition player_has_won (s : state) (p : Player) :=
+    player_active s p /\ someone_has_won s.
 
-The best I could figure out is that Dragster has been won if the branch at address 0xF39E is taken.
-I was hoping there'd be a variable that clearly says "You have won!", but I couldn't find one.
-*)
-Definition has_just_won (s : state) (p : Player) :=
-    player_active s p /\ trunc 11 (PC s) = 0x39e /\ ~~ Flag s Z.
+(*|
+How do we check the timer?
 
-Definition timer_in_hundredths (s : state) (p : Player) (t : BinNums.Z) : Prop :=
+Each player's timer is stored in binary-coded decimal, as a three-byte number.
+The first byte is in seconds, the second in hundredths, and the third in ten-thousandths of a second.
+For our level of precision, we only need the first two bytes,
+which are stored at 0x33 and 0x35 for player zero, and 0x34 and 0x36 for player one.
+|*)
+
+Definition timer_in_hundredths
+    (s : state) (p : Player) (t : BinNums.Z) : Prop :=
     exists secs hundredths,
-        is_bcd (RAM s (match p with P0 => 51 | P1 => 52 end)) secs /\
-        is_bcd (RAM s (match p with P0 => 53 | P1 => 54 end)) hundredths /\
+        is_bcd
+            (RAM s (match p with P0 => 0x33 | P1 => 0x34 end))
+            secs /\
+        is_bcd
+            (RAM s (match p with P0 => 0x35 | P1 => 0x36 end))
+            hundredths /\
         t = (hundredths + secs * 100)%Z.
 
-(* This is the claim that any speedrun of Dragster must take at least 5.57 seconds.
-The goal of this project is to prove this.
-*)
+(*|
+And at last, we can state the claim.
+|*)
+
 Definition Goal : Prop :=
-    (* Choose any valid initial state of the Atari. *)
+    (* Choose any state the Atari might have upon startup. *)
     forall s0, initial s0 ->
     (* Choose any later state, reachable from the starting state. *)
     forall s, rtc step s0 s ->
     (* Then if some player has just won, *)
-    forall p, has_just_won s p ->
-    (* Then that player's timer is a valid number, which is at least 5.57 seconds. *)
-    exists t, timer_in_hundredths s p t /\ (t >=? 557)%Z.
+    forall p, player_has_won s p ->
+    (* Then that player's timer is a valid number, *)
+    exists t, timer_in_hundredths s p t /\
+    (* which is at least 5.57 seconds. *)
+    (t >=? 557)%Z.
